simpler definition

Specification.thy
@@ -413,50 +413,26 @@ definition (in valid_graph) is_simple_path :: \<open>_ \<Rightarrow> (_,_) path 
   \<open>is_simple_path v ps v' \<longleftrightarrow> is_path v ps v' \<and> distinct (map fst ps)\<close>
 find_theorems "int_vertices"
 
-fun (in valid_graph) is_trace :: \<open>('v,'w) path \<Rightarrow> bool\<close>where \<comment> \<open>non-standard definition. Also not thoroughly thought through.\<close>
-  \<open>is_trace [] \<longleftrightarrow> V={} \<or> card V = 1\<close> |
-  \<open>is_trace ps \<longleftrightarrow> insert (snd(snd(last ps))) (int_vertices ps) = V\<close>
+definition (in valid_graph) is_trace :: \<open>('v,'w) path \<Rightarrow> bool\<close> where \<comment> \<open>non-standard definition. Also not thoroughly thought through.\<close>
+  \<open>is_trace ps \<longleftrightarrow> (if ps=[] then V={} \<or> card V = 1 else insert (snd(snd(last ps))) (int_vertices ps) = V)\<close>
 
 lemma (in valid_graph) is_trace_snoc:
   "is_trace (ps @ [p]) \<longleftrightarrow> insert (snd(snd p)) (int_vertices (ps@[p])) = V"
-  by (metis (no_types, lifting) append_is_Nil_conv is_trace.elims(2) is_trace.elims(3) last_snoc not_Cons_self2)
+  by (simp add: is_trace_def)
 
 definition (in valid_graph) is_hamiltonian_path where \<comment> \<open>or "simple trace"\<close>
   \<open>is_hamiltonian_path v ps v' \<longleftrightarrow> is_trace ps \<and> is_simple_path v ps v'\<close>
 
-fun (in valid_graph) is_hamiltonian :: \<open>('v,'w) path \<Rightarrow> bool\<close> where \<comment> \<open>to-do: unconventional intermediate definition, only for experimentation\<close>
-  \<open>is_hamiltonian [] \<longleftrightarrow> V={} \<or> card V = 1\<close> |
-  \<open>is_hamiltonian ps \<longleftrightarrow> int_vertices ps = V\<close>
+definition (in valid_graph) is_hamiltonian :: \<open>('v,'w) path \<Rightarrow> bool\<close> where \<comment> \<open>to-do: unconventional intermediate definition, only for experimentation\<close>
+  \<open>is_hamiltonian ps \<longleftrightarrow> (if ps=[] then V={} \<or> card V = 1 else int_vertices ps = V)\<close>
 
 definition (in valid_graph) is_hamiltonian_circuit where
   \<open>is_hamiltonian_circuit v ps \<longleftrightarrow> is_hamiltonian ps \<and> is_simple_path v ps v\<close>
 
 lemma (in valid_graph) is_hamiltonian_iff: "is_hamiltonian_path v ps v \<longleftrightarrow> is_hamiltonian_circuit v ps"
   apply (cases ps rule: rev_cases)
-   apply (simp_all add: is_hamiltonian_path_def is_hamiltonian_circuit_def)
-proof auto
-  fix ys :: "('v \<times> 'w \<times> 'v) list" and a :: 'v and aa :: 'w and b :: 'v
-  assume a1: "is_simple_path v (ys @ [(a, aa, b)]) v"
-  assume a2: "ps = ys @ [(a, aa, b)]"
-  assume a3: "is_trace (ys @ [(a, aa, b)])"
-  have f4: "is_path b ps b"
-    using a2 a1 by (metis (no_types) is_path.simps(1) is_path_split' is_simple_path_def)
-  have "is_trace ps"
-    using a3 a2 by meson
-  then have f5: "insert (snd (snd (last ps))) (int_vertices ps) = V \<or> ps = []"
-    using f4 is_path.elims(2) is_trace.simps(2) by blast
-  have f6: "\<forall>v ps va. ((ps = [] \<or> is_hamiltonian ps) \<or> int_vertices ps \<noteq> V) \<or> \<not> is_path va ps v"
-    using is_hamiltonian.simps(2) is_path.elims(2) by blast
-  have "ps = [] \<longrightarrow> is_hamiltonian ps"
-    using a2 by force
-  then have "is_hamiltonian ps"
-    using f6 f5 f4 by (metis fst_conv insertCI insert_absorb int_vertices_simps(2) is_path.elims(2) valid_graph.path_end valid_graph_axioms)
-  then show "is_hamiltonian (ys @ [(a, aa, b)])"
-    using a2 by meson
-qed (metis (no_types, lifting) E_validD(2) Nil_is_append_conv insert_absorb is_hamiltonian.elims(2)
-      is_path_split' is_simple_path_def last_snoc not_Cons_self2 snd_conv
-      valid_graph.is_trace.elims(3) valid_graph_axioms)
-
+   apply (simp_all add: is_hamiltonian_path_def is_hamiltonian_circuit_def is_trace_def is_hamiltonian_def is_simple_path_def)
+  by auto (metis fst_conv insert_iff int_vertices_simps(2) is_path.elims(1))
 
 term "valid_graph.is_path"
 find_theorems \<open>valid_graph.is_path\<close>
@@ -472,7 +448,7 @@ lemma is_simple_path_kon_path: \<open>kon_graph.is_simple_path a kon_path c\<clo
 
 lemma is_hamiltonian_path_kon_path: \<open>kon_graph.is_hamiltonian_path a kon_path c\<close>
   apply (simp add: kon_graph.is_hamiltonian_path_def is_simple_path_kon_path)
-  apply (simp add: kon_path_def)
+  apply (simp add: kon_path_def kon_graph.is_trace_def)
   apply eval
   done
 
@@ -482,11 +458,9 @@ lemma is_simple_path_kon_circuit: \<open>kon_graph.is_simple_path a kon_circuit 
   unfolding kon_graph.is_simple_path_def by (simp add: kon_circuit_def kon_path_def) (simp add: kon_graph_def)
 
 lemma is_hamiltonian_circuit_kon_circuit: \<open>kon_graph.is_hamiltonian_circuit a kon_circuit\<close>
-  unfolding kon_graph.is_hamiltonian_circuit_def
-  apply auto
-   apply (simp add: kon_circuit_def kon_path_def)
-   apply (simp add: kon_graph_def) apply fast
-  by (fact is_simple_path_kon_circuit)
+  unfolding kon_graph.is_hamiltonian_circuit_def kon_graph.is_hamiltonian_def
+  apply (auto simp: is_simple_path_kon_circuit)
+   by (auto simp: kon_circuit_def kon_path_def kon_graph_def)
 
 subsection \<open>Tours\<close>
 
